update typing definitions to require value argument for path type

dsn/Lang/Dynamic/FinTyping.lean
@@ -12,11 +12,70 @@ def FinTyping (e : Expr) : Typ → Prop
 | .top => Safe e
 | .iso l body => FinTyping (.extract e l) body
 | .entry l body => FinTyping (.project e l) body
-| .path left right => ∀ e' , FinTyping e' left → FinTyping (.app e e') right
+| .path left right => ∀ arg ,
+  Expr.is_value arg →
+  FinTyping arg left → FinTyping (.app e arg) right
 | .unio left right => FinTyping e left ∨ FinTyping e right
 | .inter left right => FinTyping e left ∧ FinTyping e right
 | .diff left right => FinTyping e left ∧ ¬ (FinTyping e right)
 | _ => False
+
+
+#eval Expr.pattern_match
+  (Expr.iso "hello" (Expr.record []))
+  (Pat.iso "hello" (Pat.var "x"))
+
+
+example : FinTyping (
+  Expr.app (
+    Expr.function [
+      (Pat.var "x", Expr.iso "hello" (Expr.var "x"))
+    ]
+  ) (
+    Expr.app (.function [(Pat.var "x", Expr.var "x")]) (.record [])
+  )
+) (
+  (.iso "hello" .top)
+)
+:= by
+  unfold FinTyping
+  unfold FinTyping
+  apply Or.inl
+  unfold Convergent
+  exists (.record [])
+  apply And.intro
+  { apply TransitionStar.step
+    { unfold Expr.extract
+      apply Transition.econ
+      { apply EvalCon.applicand ; exact EvalCon.hole }
+      { apply Transition.econ
+        { apply EvalCon.applicand ; exact EvalCon.hole }
+        { apply Transition.pattern_match
+          { reduce ; simp }
+          { simp [Expr.pattern_match]
+            rfl
+          }
+        }
+      }
+    }
+    { apply TransitionStar.step
+      { apply Transition.econ
+        { apply EvalCon.applicand ; exact EvalCon.hole}
+        { apply Transition.pattern_match
+          { reduce ; simp}
+          { simp [Expr.pattern_match] ; rfl }
+        }
+      }
+      { apply TransitionStar.step
+        apply Transition.pattern_match
+        { reduce ; simp}
+        { reduce ;  simp [Expr.pattern_match]; rfl }
+        { apply TransitionStar.refl }
+      }
+    }
+  }
+  { exact rfl }
+
 
 
 def Subtyping.Fin (left right : Typ) : Prop :=
@@ -65,8 +124,8 @@ mutual
 
   | path left right =>
     unfold FinTyping
-    intro h0 e'' h1
-    specialize h0 e'' h1
+    intro h0 e'' h1 h2
+    specialize h0 e'' h1 h2
     apply FinTyping.subject_reduction
     {
       have econ := EvalCon.applicator e'' .hole
@@ -147,8 +206,8 @@ mutual
 
   | path left right =>
     unfold FinTyping
-    intro h0 e'' h1
-    specialize h0 e'' h1
+    intro h0 e'' h1 h2
+    specialize h0 e'' h1 h2
     apply FinTyping.subject_expansion
     {
       have econ := EvalCon.applicator e'' .hole
@@ -405,7 +464,7 @@ end
 
 mutual
   theorem FinTyping.function_beta_reduction
-    (safe_arg : Safe arg)
+    (value_arg : Expr.is_value arg)
     (econ : EvalCon E)
     (matching : Expr.pattern_match arg p = .some eam)
   : FinTyping (E (Expr.app (Expr.function ((p, e) :: f)) arg)) t →
@@ -414,50 +473,50 @@ mutual
   | top =>
     unfold FinTyping
     intro h0
-    exact Safe.function_beta_reduction econ matching h0
+    exact Safe.function_beta_reduction value_arg econ matching h0
   | iso label body =>
     intro h0
     apply EvalCon.extract label at econ
-    apply FinTyping.function_beta_reduction safe_arg econ matching h0
+    apply FinTyping.function_beta_reduction value_arg econ matching h0
 
   | entry label body =>
     intro h0
     apply EvalCon.project label at econ
-    apply FinTyping.function_beta_reduction safe_arg econ matching h0
+    apply FinTyping.function_beta_reduction value_arg econ matching h0
 
   | path left right =>
-    intro h0 e' h1
-    specialize h0 e' h1
+    intro h0 e' h1 h2
+    specialize h0 e' h1 h2
     apply EvalCon.applicator e' at econ
-    apply FinTyping.function_beta_reduction safe_arg econ matching h0
+    apply FinTyping.function_beta_reduction value_arg econ matching h0
 
   | unio left right =>
     intro h0
     cases h0 with
     | inl h1 =>
       apply Or.inl
-      apply FinTyping.function_beta_reduction safe_arg econ matching h1
+      apply FinTyping.function_beta_reduction value_arg econ matching h1
 
     | inr h1 =>
       apply Or.inr
-      apply FinTyping.function_beta_reduction safe_arg econ matching h1
+      apply FinTyping.function_beta_reduction value_arg econ matching h1
 
   | inter left right =>
     intro h0
     have ⟨h1,h2⟩ := h0
     apply And.intro
-    { apply FinTyping.function_beta_reduction safe_arg econ matching h1 }
-    { apply FinTyping.function_beta_reduction safe_arg econ matching h2 }
+    { apply FinTyping.function_beta_reduction value_arg econ matching h1 }
+    { apply FinTyping.function_beta_reduction value_arg econ matching h2 }
 
   | diff left right =>
     intro h0
     have ⟨h1,h2⟩ := h0
     apply And.intro
-    { apply FinTyping.function_beta_reduction safe_arg econ matching h1 }
+    { apply FinTyping.function_beta_reduction value_arg econ matching h1 }
     {
       intro h3
       apply h2
-      apply FinTyping.function_beta_expansion f safe_arg econ matching h3
+      apply FinTyping.function_beta_expansion f value_arg econ matching h3
     }
 
   | _ =>
@@ -465,60 +524,60 @@ mutual
 
   theorem FinTyping.function_beta_expansion
     f
-    (safe_arg : Safe ev)
+    (value_arg : Expr.is_value arg)
     (econ : EvalCon E)
-    (matching : Expr.pattern_match ev p = .some eam)
+    (matching : Expr.pattern_match arg p = .some eam)
   : FinTyping (E (Expr.sub eam e)) t →
-    FinTyping (E (Expr.app (Expr.function ((p, e) :: f)) ev)) t
+    FinTyping (E (Expr.app (Expr.function ((p, e) :: f)) arg)) t
   := by cases t with
   | top =>
     unfold FinTyping
     intro h0
-    exact Safe.function_beta_expansion f safe_arg econ matching h0
+    exact Safe.function_beta_expansion f value_arg econ matching h0
 
   | iso label body =>
     intro h0
     apply EvalCon.extract label at econ
-    apply FinTyping.function_beta_expansion f safe_arg econ matching h0
+    apply FinTyping.function_beta_expansion f value_arg econ matching h0
 
   | entry label body =>
     intro h0
     apply EvalCon.project label at econ
-    apply FinTyping.function_beta_expansion f safe_arg econ matching h0
+    apply FinTyping.function_beta_expansion f value_arg econ matching h0
 
   | path left right =>
-    intro h0 e' h1
-    specialize h0 e' h1
+    intro h0 e' h1 h2
+    specialize h0 e' h1 h2
     apply EvalCon.applicator e' at econ
-    apply FinTyping.function_beta_expansion f safe_arg econ matching h0
+    apply FinTyping.function_beta_expansion f value_arg econ matching h0
 
   | unio left right =>
     intro h0
     cases h0 with
     | inl h1 =>
       apply Or.inl
-      apply FinTyping.function_beta_expansion f safe_arg econ matching h1
+      apply FinTyping.function_beta_expansion f value_arg econ matching h1
 
     | inr h1 =>
       apply Or.inr
-      apply FinTyping.function_beta_expansion f safe_arg econ matching h1
+      apply FinTyping.function_beta_expansion f value_arg econ matching h1
 
   | inter left right =>
     intro h0
     have ⟨h1,h2⟩ := h0
     apply And.intro
-    { apply FinTyping.function_beta_expansion f safe_arg econ matching h1 }
-    { apply FinTyping.function_beta_expansion f safe_arg econ matching h2 }
+    { apply FinTyping.function_beta_expansion f value_arg econ matching h1 }
+    { apply FinTyping.function_beta_expansion f value_arg econ matching h2 }
 
   | diff left right =>
     intro h0
     have ⟨h1,h2⟩ := h0
     apply And.intro
-    { apply FinTyping.function_beta_expansion f safe_arg econ matching h1 }
+    { apply FinTyping.function_beta_expansion f value_arg econ matching h1 }
     {
       intro h3
       apply h2
-      apply FinTyping.function_beta_reduction safe_arg econ matching h3
+      apply FinTyping.function_beta_reduction value_arg econ matching h3
     }
 
   | _ =>
@@ -550,8 +609,8 @@ mutual
     apply FinTyping.record_beta_reduction h0 h1
 
   | path left right =>
-    intro h0 h1 e' h2
-    specialize h1 e' h2
+    intro h0 h1 e' h2 h3
+    specialize h1 e' h2 h3
     apply EvalCon.applicator e' at h0
     apply FinTyping.record_beta_reduction h0 h1
 
@@ -611,8 +670,8 @@ mutual
     apply FinTyping.record_beta_expansion l h0 h1
 
   | path left right =>
-    intro h0 h1 e' h2
-    specialize h1 e' h2
+    intro h0 h1 e' h2 h3
+    specialize h1 e' h2 h3
     apply EvalCon.applicator e' at h0
     apply FinTyping.record_beta_expansion l h0 h1
 
