dsn/Lang/Dynamic/TransitionStar.lean
@@ -26,4 +26,25 @@ theorem TransitionStar.econ_preservation
   { exact ih }
 
 
+
+def Confluent (a b : Expr) :=
+  ∃ e , TransitionStar a e ∧ TransitionStar b e
+
+theorem Confluent.transitivity {a b c} :
+  Confluent a b →
+  Confluent b c →
+  Confluent a c
+:= by sorry
+
+theorem Confluent.swap {a b} :
+  Confluent a b →
+  Confluent b a
+:= by sorry
+
+theorem Confluent.app_arg_preservation {a b} f :
+  Confluent a b →
+  Confluent (.app f a) (.app f b)
+:= by sorry
+
+
 end Lang.Dynamic
