dsn/Lang/Dynamic/Safe.lean
@@ -117,72 +117,24 @@ theorem EvalCon.app_not_value
 : ¬ Expr.is_value (E (Expr.app e arg))
 := by sorry
 
-theorem Transition.econ_pattern_match_deterministic
-  (econ : EvalCon E)
-  (matching : Expr.pattern_match arg p = some eam)
-  (trans : Transition (E (Expr.app (Expr.function ((p, e) :: f)) arg)) e')
-:  e' = E (Expr.sub eam e)
-:= by sorry
-
 theorem Safe.function_beta_reduction
+  (value_arg : Expr.is_value arg)
   (econ : EvalCon E)
-  -- (safe_arg : Safe arg)
   (matching : Expr.pattern_match arg p = .some eam)
 : Safe (E (Expr.app (Expr.function ((p, e) :: f)) arg)) →
   Safe (E (Expr.sub eam e))
 := by
-  intro safe_sub
-  cases safe_sub with
-  |inl cvg_sub =>
-    apply Or.inl
-    unfold Convergent at cvg_sub
-    have ⟨e',h0,h1⟩ := cvg_sub
-    unfold Convergent
-    exists e'
-    apply And.intro
-    {
-      cases h0 with
-      | refl _ =>
-        have h2 := EvalCon.app_not_value (Expr.function ((p, e) :: f)) arg econ
-        exact False.elim (h2 h1)
-      | step e0 em e' trans trans_star =>
-        have h2 := Transition.econ_pattern_match_deterministic econ matching trans
-        rw [h2] at trans_star
-        exact trans_star
-    }
-    { exact h1 }
-  |inr dvg_sub =>
-    apply Or.inr
-    sorry
-
+  sorry
 
 theorem Safe.function_beta_expansion
   f
-  (safe_arg : Safe arg)
+  (value_arg : Expr.is_value arg)
   (econ : EvalCon E)
   (matching : Expr.pattern_match arg p = .some eam)
 : Safe (E (Expr.sub eam e)) →
   Safe (E (Expr.app (Expr.function ((p, e) :: f)) arg))
 := by
-  cases safe_arg with
-  | inl cvg_arg =>
-    intro safe_sub
-    cases safe_sub with
-    |inl cvg_sub =>
-      apply Or.inl
-      sorry
-    |inr dvg_sub =>
-      apply Or.inr
-      sorry
-  | inr dvg_arg =>
-    intro safe_sub
-    apply Or.inr
-    sorry
-
-
-
-
-
+  sorry
 
 
 
