dsn/Lang/Dynamic/Typing.lean
@@ -39,7 +39,9 @@ mutual
   | .top => Safe e
   | .iso l t => Typing am (.extract e l) t
   | .entry l t => Typing am (.project e l) t
-  | .path left right => ∀ e' , Typing am e' left → Typing am (.app e e') right
+  | .path left right => ∀ arg ,
+    Expr.is_value arg →
+    Typing am arg left → Typing am (.app e arg) right
   | .unio left right => Typing am e left ∨ Typing am e right
   | .inter left right => Typing am e left ∧ Typing am e right
   | .diff left right => Typing am e left ∧ ¬ (Typing am e right)
@@ -111,8 +113,8 @@ mutual
 
   | path left right =>
     unfold Typing
-    intro h0 e'' h1
-    specialize h0 e'' h1
+    intro h0 e'' h1 h2
+    specialize h0 e'' h1 h2
     apply Typing.subject_reduction
     {
       have econ := EvalCon.applicator e'' .hole
@@ -219,8 +221,8 @@ mutual
 
   | path left right =>
     unfold Typing
-    intro h0 e'' h1
-    specialize h0 e'' h1
+    intro h0 e'' h1 h2
+    specialize h0 e'' h1 h2
     apply Typing.subject_expansion
     {
       have econ := EvalCon.applicator e'' .hole
@@ -1329,8 +1331,8 @@ mutual
 
   | path left right =>
     unfold Typing
-    intro h0 h1 e' h2
-    specialize h1 e' h2
+    intro h0 h1 e' h2 h3
+    specialize h1 e' h2 h3
     apply EvalCon.applicator e' at h0
     apply Typing.record_beta_reduction h0 h1
 
@@ -1431,8 +1433,8 @@ mutual
 
   | path left right =>
     unfold Typing
-    intro h0 h1 e' h2
-    specialize h1 e' h2
+    intro h0 h1 e' h2 h3
+    specialize h1 e' h2 h3
     apply EvalCon.applicator e' at h0
     apply Typing.record_beta_expansion l h0 h1
 
@@ -1585,7 +1587,7 @@ theorem Subtyping.list_typ_diff_elim :
 
 mutual
   theorem Typing.function_beta_reduction
-    (safe_arg : Safe arg)
+    (value_arg : Expr.is_value arg)
     (econ : EvalCon E)
     (matching : Expr.pattern_match arg p = .some eam)
   : Typing am (E (Expr.app (Expr.function ((p, e) :: f)) arg)) t →
@@ -1597,25 +1599,25 @@ mutual
   | top =>
     unfold Typing
     intro h0
-    exact Safe.function_beta_reduction econ matching h0
+    exact Safe.function_beta_reduction value_arg econ matching h0
   | iso label body =>
     unfold Typing
     intro h0
     apply EvalCon.extract label at econ
-    apply Typing.function_beta_reduction safe_arg econ matching h0
+    apply Typing.function_beta_reduction value_arg econ matching h0
 
   | entry label body =>
     unfold Typing
     intro h0
     apply EvalCon.project label at econ
-    apply Typing.function_beta_reduction safe_arg econ matching h0
+    apply Typing.function_beta_reduction value_arg econ matching h0
 
   | path left right =>
     unfold Typing
-    intro h0 e' h1
-    specialize h0 e' h1
+    intro h0 e' h1 h2
+    specialize h0 e' h1 h2
     apply EvalCon.applicator e' at econ
-    apply Typing.function_beta_reduction safe_arg econ matching h0
+    apply Typing.function_beta_reduction value_arg econ matching h0
 
   | unio left right =>
     unfold Typing
@@ -1623,30 +1625,30 @@ mutual
     cases h0 with
     | inl h1 =>
       apply Or.inl
-      apply Typing.function_beta_reduction safe_arg econ matching h1
+      apply Typing.function_beta_reduction value_arg econ matching h1
 
     | inr h1 =>
       apply Or.inr
-      apply Typing.function_beta_reduction safe_arg econ matching h1
+      apply Typing.function_beta_reduction value_arg econ matching h1
 
   | inter left right =>
     unfold Typing
     intro h0
     have ⟨h1,h2⟩ := h0
     apply And.intro
-    { apply Typing.function_beta_reduction safe_arg econ matching h1 }
-    { apply Typing.function_beta_reduction safe_arg econ matching h2 }
+    { apply Typing.function_beta_reduction value_arg econ matching h1 }
+    { apply Typing.function_beta_reduction value_arg econ matching h2 }
 
   | diff left right =>
     unfold Typing
     intro h0
     have ⟨h1,h2⟩ := h0
     apply And.intro
-    { apply Typing.function_beta_reduction safe_arg econ matching h1 }
+    { apply Typing.function_beta_reduction value_arg econ matching h1 }
     {
       intro h3
       apply h2
-      apply Typing.function_beta_expansion f safe_arg econ matching h3
+      apply Typing.function_beta_expansion f value_arg econ matching h3
     }
 
   | exi ids quals body =>
@@ -1656,7 +1658,7 @@ mutual
     exists am'
     apply And.intro h1
     apply And.intro h2
-    apply Typing.function_beta_reduction safe_arg econ matching h3
+    apply Typing.function_beta_reduction value_arg econ matching h3
 
   | all ids quals body =>
     unfold Typing
@@ -1665,7 +1667,7 @@ mutual
     {
       intro am' dom_subset dynamic_quals
       specialize h0 am' dom_subset dynamic_quals
-      apply Typing.function_beta_reduction safe_arg econ matching h0
+      apply Typing.function_beta_reduction value_arg econ matching h0
     }
     { exact h1 }
 
@@ -1676,18 +1678,18 @@ mutual
     exists t
     exists lt_size
     apply And.intro imp_typing
-    apply Typing.function_beta_reduction safe_arg econ matching typing_body
+    apply Typing.function_beta_reduction value_arg econ matching typing_body
 
   | var id =>
     unfold Typing
     intro ⟨t, h1, h2⟩
     exists t
     apply And.intro h1
-    apply FinTyping.function_beta_reduction safe_arg econ matching h2
+    apply FinTyping.function_beta_reduction value_arg econ matching h2
 
   theorem Typing.function_beta_expansion
     f
-    (safe_arg : Safe arg)
+    (value_arg : Expr.is_value arg)
     (econ : EvalCon E)
     (matching : Expr.pattern_match arg p = .some eam)
   : Typing am (E (Expr.sub eam e)) t →
@@ -1699,26 +1701,26 @@ mutual
   | top =>
     unfold Typing
     intro h0
-    exact Safe.function_beta_expansion f safe_arg econ matching h0
+    exact Safe.function_beta_expansion f value_arg econ matching h0
 
   | iso label body =>
     unfold Typing
     intro h0
     apply EvalCon.extract label at econ
-    apply Typing.function_beta_expansion f safe_arg econ matching h0
+    apply Typing.function_beta_expansion f value_arg econ matching h0
 
   | entry label body =>
     unfold Typing
     intro h0
     apply EvalCon.project label at econ
-    apply Typing.function_beta_expansion f safe_arg econ matching h0
+    apply Typing.function_beta_expansion f value_arg econ matching h0
 
   | path left right =>
     unfold Typing
-    intro h0 e' h1
-    specialize h0 e' h1
+    intro h0 e' h1 h2
+    specialize h0 e' h1 h2
     apply EvalCon.applicator e' at econ
-    apply Typing.function_beta_expansion f safe_arg econ matching h0
+    apply Typing.function_beta_expansion f value_arg econ matching h0
 
   | unio left right =>
     unfold Typing
@@ -1726,30 +1728,30 @@ mutual
     cases h0 with
     | inl h1 =>
       apply Or.inl
-      apply Typing.function_beta_expansion f safe_arg econ matching h1
+      apply Typing.function_beta_expansion f value_arg econ matching h1
 
     | inr h1 =>
       apply Or.inr
-      apply Typing.function_beta_expansion f safe_arg econ matching h1
+      apply Typing.function_beta_expansion f value_arg econ matching h1
 
   | inter left right =>
     unfold Typing
     intro h0
     have ⟨h1,h2⟩ := h0
     apply And.intro
-    { apply Typing.function_beta_expansion f safe_arg econ matching h1 }
-    { apply Typing.function_beta_expansion f safe_arg econ matching h2 }
+    { apply Typing.function_beta_expansion f value_arg econ matching h1 }
+    { apply Typing.function_beta_expansion f value_arg econ matching h2 }
 
   | diff left right =>
     unfold Typing
     intro h0
     have ⟨h1,h2⟩ := h0
     apply And.intro
-    { apply Typing.function_beta_expansion f safe_arg econ matching h1 }
+    { apply Typing.function_beta_expansion f value_arg econ matching h1 }
     {
       intro h3
       apply h2
-      apply Typing.function_beta_reduction safe_arg econ matching h3
+      apply Typing.function_beta_reduction value_arg econ matching h3
     }
 
   | exi ids quals body =>
@@ -1759,7 +1761,7 @@ mutual
     exists am'
     apply And.intro h1
     apply And.intro h2
-    apply Typing.function_beta_expansion f safe_arg econ matching h3
+    apply Typing.function_beta_expansion f value_arg econ matching h3
 
   | all ids quals body =>
     unfold Typing
@@ -1768,7 +1770,7 @@ mutual
     {
       intro am' dom_subset dynamic_quals
       specialize h0 am' dom_subset dynamic_quals
-      apply Typing.function_beta_expansion f safe_arg econ matching h0
+      apply Typing.function_beta_expansion f value_arg econ matching h0
     }
     { exact h1 }
 
@@ -1779,14 +1781,14 @@ mutual
     exists t
     exists lt_size
     apply And.intro imp_typing
-    apply Typing.function_beta_expansion f safe_arg econ matching typing_body
+    apply Typing.function_beta_expansion f value_arg econ matching typing_body
 
   | var id =>
     unfold Typing
     intro ⟨t, h1, h2⟩
     exists t
     apply And.intro h1
-    apply FinTyping.function_beta_expansion f safe_arg econ matching h2
+    apply FinTyping.function_beta_expansion f value_arg econ matching h2
 
 
 end
@@ -1813,18 +1815,18 @@ end
 
 theorem Typing.path_intro :
   (∀ e' ,
-    Typing am e' tp →
+    Expr.is_value e' → Typing am e' tp →
     ∃ eam , Expr.pattern_match e' p = .some eam ∧ Typing am (Expr.sub eam e) tr
   ) →
   Typing am (Expr.function ((p, e) :: f)) (Typ.path (List.typ_diff tp subtras) tr)
 := by
   intro h0
   unfold Typing
-  intro e' h1
-  have h2 := Subtyping.elimination Subtyping.list_typ_diff_elim h1
-  have ⟨eam,h3,h4⟩ := h0 e' h2
-  have h5 := Typing.soundness h2
-  apply Typing.function_beta_expansion f h5 .hole h3 h4
+  intro e' h1 h2
+  have h3 := Subtyping.elimination Subtyping.list_typ_diff_elim h2
+  have ⟨eam,h4,h5⟩ := h0 e' h1 h3
+  apply Typing.function_beta_expansion f h1 .hole h4 h5
+
 
 theorem Typing.function_preservation {am p tp e f t } :
   (∀ {v} , Expr.is_value v → Typing am v tp → ∃ eam , Expr.pattern_match v p = .some eam) →
@@ -1839,9 +1841,7 @@ theorem Typing.path_elim {am ef ea t t'} :
   Typing am ea t →
   Typing am (.app ef ea) t'
 := by
-  intro h0
-  unfold Typing at h0
-  exact fun a => h0 ea a
+  sorry
 
 theorem Typing.loop_path_elim {am e t} id :
   Typing am e (.path (.var id) t) →
@@ -1961,6 +1961,25 @@ theorem Subtyping.transitivity :
   apply h1
   specialize h0 e h3
   apply h0
+
+
+
+theorem Typing.confluent_preservation {a b am t} :
+  Confluent a b →
+  Typing am a t →
+  Typing am b t
+:= by sorry
+
+theorem Typing.confluent_reflection {a b am t} :
+  Confluent a b →
+  Typing am b t →
+  Typing am a t
+:= by
+  intro h0 h1
+  apply Typing.confluent_preservation
+  apply Confluent.swap h0
+  exact h1
+
 
 
 
